\documentclass{article}
\usepackage[utf8]{inputenc}
\usepackage{amsmath}


\title{Derivatives}
\author{Reinis Freibergs}
\date{July 2021}

\begin{document}
\maketitle


\begin{equation*}
\begin{aligned}
    M(x) = Linear(W_2,b_2, ReLU( Linear(W_1,b_1,x)))=\\
    W_2\cdot ReLU(Linear(W_1,b_1,x))+b_2 =\\
    W_2\cdot (ReLU(W_1x + b_1))+b_2
\end{aligned}
\end{equation*}


\bigskip

\begin{equation*}
\begin{aligned}
    \frac{MAE(y, M(x))}{\partial b_1} = \\
    \frac{\mid y - M(x) \mid}{\partial b_1} = \\
    \frac{y - M(x)}{\mid y - M(x) \mid}\cdot \frac{-M(x)}{\partial b_1} = \\
    -\frac{y - M(x)}{\mid y - M(x)\mid}\cdot W_2\cdot \frac{ ReLU(W_1x + b ) }{\partial (W_1x + b)} = \\
    -\frac{y - M(x)}{\mid y - M(x)\mid}\cdot W_2\cdot\begin{cases}
        1, & \text{if $W_1x + b_1\geq0$}\\
        0, & \text{otherwise}
        \end{cases}
\end{aligned}
\end{equation*}

\bigskip

\begin{equation*}
\begin{aligned}
    \frac{MAE(y, M(x))}{\partial b_2} =  \\
    \frac{\mid y - M(x) \mid}{\partial b_2} = \\
    \frac{y - M(x)}{\mid y - M(x) \mid}\cdot \frac{-M(x)}{\partial b_2} =  \\
    -\frac{y - M(x)}{\mid y - M(x) \mid}
\end{aligned}
\end{equation*}


\end{document}